addBlood and discardBlood verified

dafny_verification/blood_bank.dfy
@@ -14,7 +14,15 @@ class BloodBank {
     predicate containsType(btype:string)
     reads this
     {
-        btype in blood && btype in threshold && btype in critical
+        btype in blood && btype in threshold && btype in critical &&
+        "A+" in blood && "A+" in threshold && "A+" in critical &&
+        "A-" in blood && "A-" in threshold && "A-" in critical &&
+        "B+" in blood && "B+" in threshold && "B+" in critical &&
+        "B-" in blood && "B-" in threshold && "B-" in critical &&
+        "O+" in blood && "O+" in threshold && "O+" in critical &&
+        "O-" in blood && "O-" in threshold && "O-" in critical &&
+        "AB+" in blood && "AB+" in threshold && "AB+" in critical &&
+        "AB-" in blood && "AB-" in threshold && "AB-" in critical
     }
 
     predicate isCritical(btype:string)
@@ -27,6 +35,15 @@ class BloodBank {
     constructor ()
     // modifies this;
     ensures Valid()
+    ensures "A+" in blood && "A+" in threshold && "A+" in critical
+    ensures "A-" in blood && "A-" in threshold && "A-" in critical
+    ensures "B+" in blood && "B+" in threshold && "B+" in critical
+    ensures "B-" in blood && "B-" in threshold && "B-" in critical
+    ensures "O+" in blood && "O+" in threshold && "O+" in critical
+    ensures "O-" in blood && "O-" in threshold && "O-" in critical
+    ensures "AB+" in blood && "AB+" in threshold && "AB+" in critical
+    ensures "AB-" in blood && "AB-" in threshold && "AB-" in critical
+    ensures forall i :: containsType(i) ==> blood[i] == 0 && critical[i] == true
     {
         blood := map["A+" := 0,  "A-":=0,
                      "B+" := 0,  "B-":=0,
@@ -51,9 +68,10 @@ class BloodBank {
     requires containsType(key)
     requires quantity > 0
     ensures Valid()
-    ensures key in blood ==> blood[key] == old(blood[key]) + quantity
+    ensures containsType(key) && blood[key] == old(blood[key]) + quantity
     ensures containsType(key) && blood[key] >= threshold[key] ==> !isCritical(key)
     ensures containsType(key) && blood[key] < threshold[key] ==> isCritical(key)
+    ensures containsType(key)
     {
         var amount:int := blood[key];
         var newAmount:int := amount + quantity;
@@ -138,13 +156,12 @@ class BloodBank {
 
         if !expired && !abn{
             if !added {
-                // addBlood(btype, b_amount)
+                addBlood(btype, b_amount);
             } else if blood[btype] - b_amount > 0 {
-                // discardBlood(btype, b_amount)
+                discardBlood(btype, b_amount);
             }
         }
     }
-
 }
 
 
@@ -158,5 +175,26 @@ ensures expiry <= today ==> expired == true
     } else {
         expired := true;
     }
+
+}
+
+
+method Main(){
+    var b := new BloodBank();
+
+    assert b.blood["A+"] == 0;
+    assert b.critical["A+"];
+
+    b.addBlood("A+", 300);
+    assert b.blood["A+"] == 300;
+    
+
+    b.discardBlood("A+", 290);
+    assert b.blood["A+"] == 10;
+
+    b.addBlood("A+", 5000);
+    assert b.blood["A+"] == 5010;
+
+    // b.discardBlood("A+", 5011); Fails since we're trying to discard more blood than is available
 
 }
